wip on queries_eventually_stop

systems/chord-props/QueriesEventuallyStop.v
@@ -1,8 +1,10 @@
 Require Import List.
 Import ListNotations.
+Require Import Relations.
 
 Require Import StructTact.StructTactics.
 Require Import InfSeqExt.infseq.
+Require Import InfSeqExt.classical.
 
 Require Import Chord.Chord.
 
@@ -12,9 +14,47 @@ Require Import Chord.QueryInvariant.
 
 Set Bullet Behavior "Strict Subproofs".
 
-Definition circular_wait : occurrence -> Prop.
-(* This is Ryan's problem. *)
-Admitted.
+(* The (waits_on gst) relation relates a live node h to a node s when
+   a message from h is stored in the delayed_queries list at s. *)
+Definition waits_on (gst : global_state) (h s : addr) : Prop :=
+  In h (nodes gst) /\
+  In s (nodes gst) /\
+  exists st__h st__s dstp q m,
+    sigma gst h = Some st__h /\
+    sigma gst s = Some st__s /\
+    cur_request st__h = Some (dstp, q, m) /\
+    addr_of dstp = s /\
+    In (h, m) (delayed_queries st__s).
+
+(* There is a cycle in a relation iff there's an element related to
+   itself by the transitive closure of the relation. *)
+Definition has_cycle {A : Type} (R : A -> A -> Prop) : Prop :=
+  exists x,
+    clos_trans_1n A R x x.
+
+(* A circular wait (in a given state) is a cycle in the waits_on
+   relation (for that state). *)
+Definition circular_wait (occ : occurrence) : Prop :=
+  has_cycle (waits_on (occ_gst occ)).
+
+Inductive fin_chain {A : Type} (R : A -> A -> Prop) : list A -> Prop :=
+| FinChainNil : fin_chain R []
+| FinChainOne : forall x, fin_chain R [x]
+| FinChainCons : forall x y l,
+    R x y ->
+    fin_chain R (y :: l) ->
+    fin_chain R (x :: y :: l).
+
+Theorem pigeon_cycle :
+  forall A (R : A -> A -> Prop) l,
+    (forall a b, R a b -> In a l /\ In b l) ->
+    forall c,
+    fin_chain R c ->
+    length c > length l ->
+    has_cycle R.
+Proof.
+(* not sure I need this machinery yet *)
+Abort.
 
 Definition busy_if_live (h : addr) (occ : occurrence) :=
   forall st,
@@ -27,6 +67,50 @@ Definition not_busy_if_live (h : addr) (occ : occurrence) :=
     live_node (occ_gst occ) h ->
     sigma (occ_gst occ) h = Some st ->
     cur_request st = None.
+
+Theorem never_stopping_means_stuck_on_a_single_query :
+  forall ex h,
+    lb_execution ex ->
+    reachable_st (occ_gst (hd ex)) ->
+    strong_local_fairness ex ->
+    live_node (occ_gst (hd ex)) h ->
+    forall st dstp q m,
+      sigma (occ_gst (hd ex)) h = Some st ->
+      cur_request st = Some (dstp, q, m) ->
+      always (~_ (now circular_wait)) ex ->
+      always (now (fun o => forall st',
+                           sigma (occ_gst o) h = Some st' /\
+                           cur_request st' <> None)) ex ->
+      exists dstp' q' m',
+        continuously (now (fun o =>
+                             forall st',
+                               sigma (occ_gst o) h = Some st' ->
+                               cur_request st' = Some (dstp', q', m')))
+                     ex.
+Proof.
+Admitted.
+
+Theorem stuck_on_a_single_query_means_target_is_too :
+  forall ex h,
+    lb_execution ex ->
+    reachable_st (occ_gst (hd ex)) ->
+    strong_local_fairness ex ->
+    live_node (occ_gst (hd ex)) h ->
+    forall dstp q m,
+      always (now
+                (fun o =>
+                   forall st,
+                     sigma (occ_gst o) h = Some st ->
+                     cur_request st = Some (dstp, q, m)))
+             ex ->
+    exists dstp' q' m',
+      continuously (now (fun o =>
+                           forall st',
+                             sigma (occ_gst o) (addr_of dstp') = Some st' ->
+                             cur_request st' = Some (dstp', q', m')))
+                   ex.
+Proof.
+Admitted.
 
 Theorem queries_eventually_stop' :
   forall ex h,
